1.

2.

10.

$
设c^2=||u-v||^2,a^2=||u||^2以及b^2=||v||^2.
$
$||u-v||^2=||u||^2+||v||^2-2|u||v|cos(\theta).$

$|u||v|cos(\theta)=\frac{||u||^2+||v||^2-||u-v||^2}{2}$

$|u||v|cos(\theta)=\frac{u_x^2+u_y^2+u_z^2+v_x^2+v_y^2+v_z^2-(u_x-v_x)^2-(u_y-v_y)^2-(u_z-u_z)^2}{2}$


$|u||v|cos(\theta)=u_xv_x+u_yv_y+u_zv_z$

14.

$||u\times v||=||u||*||v||*sin(\theta)$

$||(u_yv_z-u_zv_y,u_zv_x-u_xv_z,u_xv_y-u_yv_x)||=||u||*||v||*sin(\theta)$


$||(u_yv_z-u_zv_y,u_zv_x-u_xv_z,u_xv_y-u_yv_x)||^2=||u||^2*||v||^2*sin(\theta)^2$

$(u_yv_z-u_zv_y)^2+(u_zv_x-u_xv_z)^2+(u_xv_y-u_yv_x)^2=(u_x^2+u_y^2+u_z^2)*(v_x^2+v_y^2+v_z^2)*sin(\theta)^2$

$(u_yv_z-u_zv_y)^2+(u_zv_x-u_xv_z)^2+(u_xv_y-u_yv_x)^2=(u_x^2+u_y^2+u_z^2)*(v_x^2+v_y^2+v_z^2)*(1-cos(\theta)^2)$

$(u_yv_z-u_zv_y)^2+(u_zv_x-u_xv_z)^2+(u_xv_y-u_yv_x)^2=(u_x^2+u_y^2+u_z^2)*(v_x^2+v_y^2+v_z^2)*(1-\frac{u_x^2v_x^2+u_y^2v_y^2+u_z^2v_z^2}{(u_x^2+u_y^2+u_z^2)(v_x^2+v_y^2+v_z^2)})$